@prefix owl: <http://www.w3.org/2002/07/owl#> .
@prefix rdfs: <http://www.w3.org/2000/01/rdf-schema#> .
@prefix xsd: <http://www.w3.org/2001/XMLSchema#> .
@prefix ids: <https://w3id.org/idsa/core/> .


# Classes
# -------

ids:App
    a owl:Class;
    rdfs:label "App"@en;
    rdfs:comment "Self-contained, self-descriptive software package that is distributed via the App Store and deployed inside a Connector; provides access to data and data processing capaÂ­bilities; the interface of a Data App is semantically described by the IDS Information Model."@en;
    # TODO: exposes at least one interface
.

ids:appDocumentation
    a owl:DatatypeProperty ;
    rdfs:domain ids:App ;
    rdfs:range xsd:string ;
    rdfs:label "app documentation"@en ;
    rdfs:comment "text documentation of the data app"@en ;
.

ids:endpointBinding
    a owl:ObjectProperty;
    rdfs:label "endpoint binding"@en ;
    rdfs:domain ids:App;
    rdfs:range ids:EndpointBinding;
    rdfs:comment "Endpoint protocol bindings of a data app"@en ;
.

ids:supportedUsagePolicies a owl:ObjectProperty ;
	rdfs:domain ids:App ;
	rdfs:range ids:UsagePolicyClass ;
	rdfs:label "supported usage policies" @en;
	rdfs:comment "IDS Usage Policies a App supports"@en;
.
	
ids:appType a owl:ObjectProperty ;
	rdfs:domain ids:App ;
	rdfs:range ids:AppType ;
	rdfs:label "data app type"@en;
	rdfs:comment "The category of the data app. Class ids:AppType contains a controlled vocabulary of categories."@en;
.

ids:appContainerSpecReference: 
    a owl:DatatypeProperty ;
    rdfs:domain ids:App ;
    rdfs:range xsd:anyURI ;
	rdfs:label "api container spec reference"@en ;
    rdfs:comment "Reference to the container specification of the ids:App, e.g., reference to docker build files."@en ;
.

ids:appContainerSpec
    a owl:DatatypeProperty ;
    rdfs:domain ids:App ;
    rdfs:range xsd:string ;
	rdfs:label "api container spec"@en ;
    rdfs:comment "The container specification of the ids:App, e.g., docker build files. It is recommended to use the ids:appContainerSpecReference property. This property should be used, when it is not possible to refer to a container specification using IRIs."@en ;
.