@prefix dct: <http://purl.org/dc/terms/> .
@prefix dcat: <http://www.w3.org/ns/dcat#> .
@prefix ids: <https://w3id.org/idsa/core/> .

@prefix owl: <http://www.w3.org/2002/07/owl#> .
@prefix rdf:   <http://www.w3.org/1999/02/22-rdf-syntax-ns#> .
@prefix rdfs: <http://www.w3.org/2000/01/rdf-schema#> .
@prefix xsd: <http://www.w3.org/2001/XMLSchema#> .
@prefix odrl: <http://www.w3.org/ns/odrl/2/> .

# Classes
# -------

ids:AssetCollection
    a owl:Class;
    rdfs:subClassOf odrl:Asset, odrl:AssetCollection ;
    rdfs:label "Asset Collection"@en ;
    rdfs:comment "An AssetCollection is a bracket object combining several odrl:Asset."@en;
.


# Properties
# ----------

ids:assetSource a owl:ObjectProperty ;
    rdfs:subPropertyOf odrl:source ;
    rdfs:label "asset source"@en ;
    rdfs:domain ids:AssetCollection ;
    rdfs:range xsd:anyURI ;
    rdfs:comment "A remote link to the location (PIP) where this AssetCollection and its members are maintained."@en ;
.

# united with ids:assetRefinement of the ids:Rule class.
#ids:assetRefinement a owl:ObjectProperty ;
#    rdfs:subPropertyOf odrl:refinement ;
#    rdfs:label "asset refinement"@en ;
#    rdfs:domain ids:AssetCollection ;
#    rdfs:range ids:AbstractConstraint ;
#    rdfs:comment "Conditions which specify whether an arbitrary odrl:Asset is a member of this AssetCollection."@en ;
#.
