@prefix owl: <http://www.w3.org/2002/07/owl#> .
@prefix rdfs: <http://www.w3.org/2000/01/rdf-schema#> .
@prefix dct: <http://purl.org/dc/terms/> .
@prefix ids: <https://w3id.org/idsa/core/> .
@prefix xsd: <http://www.w3.org/2001/XMLSchema#> .
@prefix idsm: <https://w3id.org/idsa/metamodel/> .

# Classes
# -------

ids:MediaType
    a owl:Class;
    rdfs:subClassOf dct:MediaType ; # *not* restricted to IANA media types
    rdfs:label "Media Type"@en ;
    rdfs:comment "General class of media types (formerly known as MIME types)." ;
    idsm:usage "ids:GeneralMediaType is used only when no ids:IANAMediaType available."@en ;
    idsm:abstract true;
    .

ids:GeneralMediaType
    a owl:Class ;
    rdfs:subClassOf ids:MediaType;
    rdfs:label "General Media Type"@en ;
    rdfs:comment "A selection of general media types to be used for data published on the IDS when no IANA type is available.".

ids:IANAMediaType
    a owl:Class ;
    rdfs:subClassOf ids:MediaType;
    rdfs:label "IANA Media Type"@en ;
    rdfs:comment "The class of media types registered with IANA.";
    rdfs:seeAlso <https://www.iana.org/assignments/media-types/> ; # authoritative IANA list
    rdfs:seeAlso <http://www.sparontologies.net/mediatype/> ; # RDF description of IANA-registered media types
    rdfs:seeAlso <http://dx.doi.org/10.6084/m9.figshare.1608294> ; # downloadable archive of SPAR Media Type ontology
    idsm:usage "Definition of an ids:IANAMediaType should define individual equivalence to corresponding SPAR-Media Type."@en ;
    idsm:example
"""
    idsc_media:TEXT_CSV
        a ids:IANAMediaType;
        # the retrieved representation (HTML, turtle, RDF/XML) depends on content negotiation
        owl:sameAs <https://w3id.org/spar/mediatype/text/csv> .
""";
    .

# Properties
# ----------

#ids:magicNumber
#    a owl:DatatypeProperty ;
#    rdfs:label "magic number"@en ;
#    rdfs:label "file signature"@en ;
#    rdfs:domain ids:MediaType ;
#    rdfs:range xsd:string ;
#    rdfs:comment "Alphanumeric sequence (located within a file) used to identify the file format."@en ;
#    rdfs:seeAlso <https://en.wikipedia.org/wiki/File_format#Magic_number> ;
#    .

ids:filenameExtension
    # similar to <http://dbpedia.org/property/extension>, but does not contain dot separator
    a owl:DatatypeProperty ;
    rdfs:label "filename extension"@en ;
    # rdfs:label "Dateiendung"@de ;
    rdfs:domain ids:MediaType ;
    rdfs:range xsd:string ;
    rdfs:comment "Suffix of a file name, typically separated by a period, indicating the nature and intended processing of the file."@en ;
    rdfs:seeAlso <https://en.wikipedia.org/wiki/Filename_extension> ;
    .

