@prefix owl: <http://www.w3.org/2002/07/owl#> .
@prefix rdfs: <http://www.w3.org/2000/01/rdf-schema#> .
@prefix dct: <http://purl.org/dc/terms/> .
@prefix xsd: <http://www.w3.org/2001/XMLSchema#> .
@prefix odrl: <http://www.w3.org/ns/odrl/2/> .
@prefix ids: <https://w3id.org/idsa/core/> .


# Classes
# -------

ids:UsageControlObject a owl:Class;
           rdfs:label "Usage Control Object"@en;
           rdfs:comment "A data element containing all relevant information for usage control engines."@en;
           .

 # Properties
 # ----------

 ids:data a owl:ObjectProperty;
          rdfs:label "has data"@en;
          rdfs:domain ids:UsageControlObject;
          rdfs:range xsd:anyURI ;
          rdfs:comment "The related data or a pointer/reference to it."@en ;
 .

 ids:user a owl:ObjectProperty;
         rdfs:label "has user"@en;
         rdfs:domain ids:UsageControlObject;
         rdfs:range ids:Participant ;
         rdfs:comment "The participant intending to use the data."@en ;
 .

 ids:source a owl:ObjectProperty;
          rdfs:label "source"@en;
          rdfs:domain ids:UsageControlObject;
          rdfs:range xsd:anyURI ;
          rdfs:comment "The application which provided the data object. Should be a valid URI. Must be unique in the regarded environment."@en ;
 .

 ids:contract a owl:ObjectProperty;
          rdfs:label "has contract"@en;
          rdfs:domain ids:UsageControlObject;
          rdfs:range ids:ContractAgreement ;
          rdfs:comment "The target contract defining the usage of the data object."@en ;
 .


 ids:usageDuration a owl:ObjectProperty;
         rdfs:label "usage duration"@en;
         rdfs:domain ids:UsageControlObject;
         rdfs:range xsd:duration ;
         rdfs:comment "Duration, which this asset is in use by now. Might be calculated on the fly when requested by a Usage Control Engine."@en ;
 .

 ids:accessed a owl:ObjectProperty;
         rdfs:label "last accessed"@en;
         rdfs:domain ids:UsageControlObject;
         rdfs:range xsd:dateTimeStamp ;
         rdfs:comment "Last read or write access."@en ;
 .

 # united with ids:action of the ids:Rule class.
 # ids:action a owl:ObjectProperty;
 #        rdfs:label "applied actions"@en;
 #        rdfs:domain ids:UsageControlObject;
 #        rdfs:range ids:Action ;
 #        rdfs:comment "The sequence of executed actions on the data object. Must be an element of ids:Action."@en ;
 #.

 ids:hasState a owl:ObjectProperty;
         rdfs:label "has state"@en;
         rdfs:domain ids:UsageControlObject;
         rdfs:range ids:ArtifactState ;
         rdfs:comment "The list of combined current states of the data object."@en ;
 .

 ids:requester a owl:ObjectProperty;
         rdfs:label "requesting application"@en;
         rdfs:domain ids:UsageControlObject;
         rdfs:range xsd:anyURI ;
         rdfs:comment "	The target application requesting the usage. Should be some locally unique identifiers, preferably URIs."@en ;
 .
