@prefix dct: <http://purl.org/dc/terms/> .
@prefix dcat: <http://www.w3.org/ns/dcat#> .
@prefix ids: <https://w3id.org/idsa/core/> .
@prefix idsm: <https://w3id.org/idsa/metamodel/> .
@prefix owl: <http://www.w3.org/2002/07/owl#> .
@prefix rdf:   <http://www.w3.org/1999/02/22-rdf-syntax-ns#> .
@prefix rdfs: <http://www.w3.org/2000/01/rdf-schema#> .
@prefix xsd: <http://www.w3.org/2001/XMLSchema#> .
@prefix sh: <http://www.w3.org/ns/shacl#> .
@prefix void: <http://rdfs.org/ns/void#> .


ids:VocabularyData a owl:Class;
    rdfs:subClassOf void:Dataset;
    rdfs:label "VocabularyData."@en ;
    rdfs:comment "Class for Vocabularies used to describe domain-specific ids:Resources and ids:Representations."@en;
    rdfs:seeAlso <https://www.w3.org/TR/vocab-dcat/#class-dataset>;
    idsm:validation [
        idsm:forProperty ids:propertyPartition;
        idsm:relationType idsm:OneToMany;
    ];
    idsm:validation [
        idsm:forProperty ids:property;
        idsm:relationType idsm:OneToMany;
    ];
.

ids:vocabulary a owl:DatatypeProperty;
    rdfs:subPropertyOf void:vocabulary;
    rdfs:domain ids:VocabularyData ;
    rdfs:range xsd:anyURI ;
    rdfs:label "vocabulary"@en;
    rdfs:comment "Refrence to an URI with the domain vocabulary."@en.

ids:propertyPartition a owl:ObjectProperty;
    rdfs:subPropertyOf void:propertyPartition;
    rdfs:domain ids:VocabularyData ;
    rdfs:range ids:VocabularyData ;
    rdfs:label "propertyPartition"@en;
    rdfs:comment "A subset of a ids:VocabularyDataset that contains only the triples of a certain property."@en.

ids:property a owl:DatatypeProperty;
    rdfs:subPropertyOf void:property;
    rdfs:domain ids:VocabularyData ;
    rdfs:range xsd:string ;         # pointing to rdf:Property (how void does) may lead to problems during transformation to code library.
    rdfs:label "property"@en;
    rdfs:comment "The rdf:Property that is the predicate of all triples in a property-based partition.."@en.
