@prefix owl: <http://www.w3.org/2002/07/owl#> .
@prefix rdf: <http://www.w3.org/1999/02/22-rdf-syntax-ns#> .
@prefix rdfs: <http://www.w3.org/2000/01/rdf-schema#> .
@prefix xsd: <http://www.w3.org/2001/XMLSchema#> .
@prefix dct: <http://purl.org/dc/terms/> .
@prefix ids: <https://w3id.org/idsa/core/> .
@prefix idsm: <https://w3id.org/idsa/metamodel/> .

# Classes
# -------

ids:Endpoint a owl:Class ;
    idsm:abstract true;
    rdfs:label "Endpoint"@en ;
    rdfs:comment "Access point of data exchange and service interaction."@en ;
    idsm:validation [
        idsm:forProperty ids:endpointHost;
        idsm:constraint idsm:NotNull;
    ];
    idsm:validation [
        idsm:forProperty ids:path;
        idsm:constraint idsm:NotNull;
    ] . 

ids:StaticEndpoint
    a owl:Class ;
    rdfs:subClassOf ids:Endpoint ;
    rdfs:label "Static Endpoint"@en ;
    rdfs:comment "Endpoint exposing an Artifact."@en ;
    idsm:validation [
        idsm:forProperty ids:endpointArtifact;
        idsm:constraint idsm:NotNull;
    ] ;
    owl:disjointWith ids:InteractiveEndpoint .

ids:InteractiveEndpoint
    a owl:Class ;
    rdfs:subClassOf ids:Endpoint ;
    rdfs:label "Interactive Endpoint"@en ;
    rdfs:comment "Endpoint exposing a digital content in an interactive way."@en ;
    idsm:validation [
        idsm:forProperty ids:endpointOperationBinding;
        idsm:constraint idsm:NotNull;
    ] ;
    owl:disjointWith ids:StaticEndpoint .

#ids:DataSink
#    a owl:Class ;
#    rdfs:subClassOf ids:Endpoint ;
#    idsm:abstract true ;
#    rdfs:label "Data Sink"@en ;
#    rdfs:comment "Endpoint consuming digital content supplied by a Data Provider."@en.

#ids:DataSource
#    a owl:Class ;
#    rdfs:subClassOf ids:Endpoint ;
#    idsm:abstract true ;
#    rdfs:label "Data Source"@en ;
#    rdfs:comment "Endpoint providing digital content for being retrieved or subscribed to by a Data Consumer."@en.

# Properties of Endpoint
# ----------------------

ids:endpointHost
    a owl:ObjectProperty;
    rdfs:label "endpoint host"@en;
    rdfs:domain ids:Endpoint;
    rdfs:range ids:Host;
    rdfs:comment "Network host that exposes resource content and Connector services via this endpoint."@en ;
    idsm:explanation
"""Definition of a Resource Endpoint is by purpose split into an address part (path, topic etc.)
and host information used to augment and resolve the address. As such, the overall address space
is self-contained and may move across hosts. Further, changes of either component (address vs. host)
do not affect the other."""@en
    .

ids:endpointArtifact
    a owl:ObjectProperty;
    rdfs:label "endpoint artifact"@en;
    rdfs:domain ids:StaticEndpoint;
    rdfs:range ids:Artifact;
    rdfs:comment "Content instance mediated via this individual endpoint (1:1 mapping)."@en.

ids:endpointOperationBinding
    a owl:ObjectProperty;
    rdfs:label "endpoint operation binding"@en;
    rdfs:domain ids:InteractiveEndpoint;
    rdfs:range ids:OperationBinding;
    rdfs:comment "Operation bound to the endpoint by means of a protocol binding."@en.

ids:path
    a owl:DatatypeProperty;
    rdfs:label "path"@en;
    rdfs:domain ids:Endpoint;
    rdfs:range xsd:string;
    rdfs:comment "Relative path, topic or queue at which the content is published by the related host."@en.
    # The property is mandatory for Artifact exposing Endpoints i.e. the only discriminating element
    # TODO: Discuss completeness requirement - is the path required to be complete / self-contained or does it combine with Artifact/@fileName suffix?

ids:inboundPath
    a owl:DatatypeProperty;
    rdfs:label "inbound topic"@en;
    rdfs:domain ids:Endpoint;
    rdfs:range xsd:string;
    rdfs:comment "Relative path used for inbound communication via this endpoint, i.e. input messages and faults only."@en.

ids:outboundPath
    a owl:DatatypeProperty;
    rdfs:label "outbound topic"@en;
    rdfs:domain ids:Endpoint;
    rdfs:range xsd:string;
    rdfs:comment "Relative path used for outbound communication via this endpoint, i.e. output messages and faults only."@en.

