@prefix owl: <http://www.w3.org/2002/07/owl#> .
@prefix rdfs: <http://www.w3.org/2000/01/rdf-schema#> .
@prefix dct: <http://purl.org/dc/terms/> .
@prefix xsd: <http://www.w3.org/2001/XMLSchema#> .
@prefix odrl: <http://www.w3.org/ns/odrl/2/> .
@prefix ids: <https://w3id.org/idsa/core/> .
@prefix idsm: <https://w3id.org/idsa/metamodel/> .

# Classes
# -------

ids:PaymentModel
    a owl:Class ;
    rdfs:label "Payment model"@en;
    rdfs:comment "Model considering the type and timing of the payment (the effective financial compensation)."@en ;
    idsm:abstract true .

# Distinction by payment timing
#
ids:ImmediatePayment
    a owl:Class ;
    rdfs:subClassOf ids:PaymentModel ;
    rdfs:label "Immediate payment"@en;
    rdfs:comment "Payment taking place immediately before or simultaneously to product consumption."@en ;
    idsm:abstract true .

ids:SubscriptionPayment # TODO: Reword
    a owl:Class ;
    rdfs:subClassOf ids:PaymentModel ;
    rdfs:label "Subscription payment"@en;
    rdfs:comment "Payment taking on periodical rate according to underlying contract terms."@en ;
    owl:disjointWith ids:ImmediatePayment .

# Distinction by type of payment
#
ids:CashMachine # Pattern: Cash machine
    a owl:Class ;
    rdfs:subClassOf ids:ImmediatePayment ;
    rdfs:label "Cash machine"@en;
    rdfs:comment "e.g. Paypal, Visa Card"@en .

ids:PrePaidCredit
    a owl:Class ;
    rdfs:subClassOf ids:ImmediatePayment ;
    rdfs:label "Pre-paid payment"@en;
    rdfs:comment "e.g. prepaid SIM"@en .

ids:PostPaidCredit
    a owl:Class ;
    rdfs:subClassOf ids:SubscriptionPayment ;
    rdfs:label "Post-paid payment"@en;
    rdfs:comment "Payment method requiring a contract allowing the product provider to charge the subscriber."@en .

