@prefix idsm: <https://w3id.org/idsa/metamodel/> .
@prefix owl: <http://www.w3.org/2002/07/owl#> .
@prefix rdf: <http://www.w3.org/1999/02/22-rdf-syntax-ns#> .
@prefix rdfs: <http://www.w3.org/2000/01/rdf-schema#> .
@prefix skos: <http://www.w3.org/2004/02/skos/core#> .
@prefix xsd: <http://www.w3.org/2001/XMLSchema#> .
@prefix vann: <http://vocab.org/vann/> .

# Properties
# ----------

idsm:abstract
    a owl:DatatypeProperty;
    rdfs:label "abstract"@en;
    rdfs:domain owl:Class;
    rdfs:range xsd:boolean;
    rdfs:comment "Abstract concept marker, its instantiation is delegated to extending constructs (sub-classes or sub-properties)."@en.

idsm:referenceByUri
    a owl:DatatypeProperty;
    rdfs:label "Reference by URL"@en;
    rdfs:domain owl:Class;
    rdfs:range xsd:boolean;
    rdfs:comment "States that a reference to a class should not be implemented by a local in-memory reference but as a URL addressing the remote instance."@en.

# annotation properties
# - generic domain rdfs:Resource applies to any classes and predicates
# - language-tagged text, rdf:PlainLiteral

# bad practice for RDF properties
#idsm:labelPluralForm
#    a owl:DatatypeProperty;
#    rdfs:subPropertyOf skos:prefLabel;
#    rdfs:label "plural label form"@en;
#    rdfs:domain rdfs:Resource;
#    rdfs:range rdf:PlainLiteral;
#    rdfs:comment "The preferred lexical label for a resource, in plural form in a given language."@en.

idsm:example
    a owl:DatatypeProperty;
    # not extending vann:example because derived from rdfs:seeAlso with range rdfs:Resource
    rdfs:label "example"@en;
    rdfs:domain rdfs:Resource;
    rdfs:range rdfs:Resource ;
    rdfs:comment "Literal in-line example of instantiating given modeling construct."@en .

idsm:usage
    a owl:DatatypeProperty;
    # not extending vann:usageNote for same reason (*reference to* an explanatory resource)
    rdfs:label "usage"@en;
    rdfs:domain rdfs:Resource;
    rdfs:range rdf:PlainLiteral;
    rdfs:comment "Literal in-line note recommending a particular usage of given modeling construct."@en .

idsm:rationale
    a owl:DatatypeProperty;
    rdfs:label "rationale"@en;
    rdfs:domain rdfs:Resource;
    rdfs:range rdf:PlainLiteral;
    rdfs:comment "Literal description of motivations, requirements and design decisions underlying the modeling of a construct."@en.

idsm:competencyQuestion
    a owl:DatatypeProperty;
    rdfs:label "competency question"@en;
    rdfs:domain rdfs:Resource;
    rdfs:range rdf:PlainLiteral;
    rdfs:comment "Single 'competency question' the modeling construct is intended to address."@en ;
    rdfs:seeAlso <https://protege.stanford.edu/publications/ontology_development/ontology101-noy-mcguinness.html#Step1> .

idsm:issue
    a owl:DatatypeProperty;
    rdfs:label "issue"@en;
    rdfs:domain rdfs:Resource;
    rdfs:range rdf:PlainLiteral;
    rdfs:comment "Explicit statement of pending issue related to the resource."@en .
