@prefix rdf:   <http://www.w3.org/1999/02/22-rdf-syntax-ns#> .
@prefix owl: <http://www.w3.org/2002/07/owl#> .
@prefix rdfs: <http://www.w3.org/2000/01/rdf-schema#> .
@prefix xsd: <http://www.w3.org/2001/XMLSchema#> .
@prefix dcat: <http://www.w3.org/ns/dcat#> .
@prefix ids: <https://w3id.org/idsa/core/> .
@prefix idsm: <https://w3id.org/idsa/metamodel/> .

# Classes
# -------

ids:Host
    a owl:Class;
    rdfs:label "Host"@en ;
    rdfs:comment "Network host capable of serving and consuming digital content and services."@en;
    idsm:validation [
        idsm:forProperty ids:protocol;
        idsm:constraint idsm:NotNull;
    ];
    idsm:validation [
        idsm:forProperty ids:accessUrl;
        idsm:constraint idsm:NotNull;
    ].


#ids:ConnectionOption a owl:Class;
#    rdfs:label "ConnectionOption"@en ;
#    rdfs:comment "Class that aggregates Protocol types and URLs and Paths for using them for InfrastructureComponent interactions."@en.

# Properties
# ----------

ids:protocol a owl:ObjectProperty;
    rdfs:domain ids:Host;
    rdfs:range ids:Protocol ;
    rdfs:label "protocol"@en;
    rdfs:comment "Communication protocol supported by the host."@en.

ids:accessUrl
    a owl:DatatypeProperty;
    rdfs:domain ids:Host;
    rdfs:range xsd:anyURI ;
    rdfs:label "Access URL"@en;
    rdfs:comment "Access URL (e.g., http/websocket host, mqtt broker address and port) required for communication using the protocol."@en ;
    rdfs:seeAlso <https://github.com/mqtt/mqtt.github.io/wiki/URI-Scheme> .
    # https://example.org:8080
    # mqtts://198.41.30.241:8883

ids:pathPrefix # optional
    a owl:DatatypeProperty;
    rdfs:label "path prefix"@en;
    rdfs:domain ids:Host;
    rdfs:range xsd:string;
    rdfs:comment "Prefix optionally prepended to all of the paths served by the host."@en.

