@prefix owl: <http://www.w3.org/2002/07/owl#> .
@prefix rdf: <http://www.w3.org/1999/02/22-rdf-syntax-ns#> .
@prefix rdfs: <http://www.w3.org/2000/01/rdf-schema#> .
@prefix xsd: <http://www.w3.org/2001/XMLSchema#> .
@prefix dct: <http://purl.org/dc/terms/> .
@prefix ids: <https://w3id.org/idsa/core/> .
@prefix idsm: <https://w3id.org/idsa/metamodel/> .

# Classes
# -------

ids:Operation a owl:Class;
    rdfs:subClassOf ids:Described;
    rdfs:label "Operation"@en;
    rdfs:comment "Building block of an Interface; describes the interaction by defining input, output and error parameters."@en;
    idsm:abstract true;
    idsm:validation [
        idsm:forProperty ids:input;
        idsm:relationType idsm:OneToMany;
    ];
    idsm:validation [
        idsm:forProperty ids:output;
        idsm:relationType idsm:OneToMany;
    ];
    idsm:validation [
        idsm:forProperty ids:fault;
        idsm:relationType idsm:OneToMany;
    ].

# Properties for describing an Operation
# --------------------------------------

ids:operationType
    a owl:ObjectProperty;
    rdfs:domain ids:Operation;
    rdfs:range ids:OperationType;
    rdfs:label "operation type"@en;
    rdfs:comment "Detailed type, genre or interpretation of the Operation."@en.

ids:pattern
    a owl:ObjectProperty;
    rdfs:domain ids:Operation;
    rdfs:range ids:MessageExchangePattern;
    rdfs:label "pattern"@en;
    rdfs:comment "Reference to Message Exchange Pattern supported by the operation."@en.

ids:input a owl:ObjectProperty;
    rdfs:domain ids:Operation;
    rdfs:range ids:Parameter;
    rdfs:label "input"@en;
    rdfs:comment "Reference to an input Parameter (optionaly) used by the Operation."@en.

ids:mandatoryInput
    a owl:ObjectProperty;
    rdfs:subPropertyOf ids:input;
    rdfs:domain ids:Operation;
    rdfs:range ids:Parameter;
    rdfs:label "mandatoryInput"@en;
    rdfs:comment "Reference to an input Parameter required by the Operation."@en.

ids:inputGroup a owl:ObjectProperty;
    rdfs:domain ids:Operation;
    rdfs:range ids:ParameterGroup;
    rdfs:label "input group"@en;
    rdfs:comment "Parameterizes the input of an Operation with a predefined paramter group."@en.

ids:mandatoryInputGroup a owl:ObjectProperty;
    rdfs:domain ids:Operation;
    rdfs:range ids:ParameterGroup;
    rdfs:label "mandatory input group"@en;
    rdfs:comment "Parameterizes the input of an Operation with a predefined mandatory parameter group."@en.

ids:output a owl:ObjectProperty;
    rdfs:domain ids:Operation;
    rdfs:range ids:Parameter;
    rdfs:label "output"@en;
    rdfs:comment "Holds the result of an Operation."@en.

ids:mandatoryOutput a owl:ObjectProperty;
    rdfs:subPropertyOf ids:output;
    rdfs:domain ids:Operation;
    rdfs:range ids:Parameter;
    rdfs:label "mandatoryOutput"@en;
    rdfs:comment "Holds the mandatory result of an Operation."@en.

ids:fault a owl:ObjectProperty;
    rdfs:domain ids:Operation;
    rdfs:range ids:Parameter;
    rdfs:label "fault"@en;
    rdfs:comment "Holds information when an Operation has failed."@en.

# TODO: Replace by general annotation
#
#ids:operationLabel rdfs:subPropertyOf rdfs:label;
#    a owl:DatatypeProperty;
#    rdfs:domain ids:Operation;
#    rdfs:range rdf:PlainLiteral;
#    rdfs:label "Operation Label"@en;
#    rdfs:comment "Freetext label of the Operation as it should be shown in public indexes."@en.

#ids:operationDescription rdfs:subPropertyOf dct:description;
#    a owl:DatatypeProperty;
#    rdfs:domain ids:Operation;
#    rdfs:range rdf:PlainLiteral;
#    rdfs:label "Operation Description"@en;
#    rdfs:comment "Freetext description of the Operation as it should be shown in public indexes."@en.

