@prefix owl: <http://www.w3.org/2002/07/owl#> .
@prefix rdf: <http://www.w3.org/1999/02/22-rdf-syntax-ns#> .
@prefix rdfs: <http://www.w3.org/2000/01/rdf-schema#> .
@prefix xsd: <http://www.w3.org/2001/XMLSchema#> .
@prefix dct: <http://purl.org/dc/terms/> .
@prefix ids: <https://w3id.org/idsa/core/> .
@prefix idsm: <https://w3id.org/idsa/metamodel/> .

# Classes
# -------

# Parameter is a re-usable for in/out/fault, usage indicated by predicates
# purpose/interpretation is not necessarily re-usable, e.g. startDate vs. endDate
# default cardinality: {0,1} (because fault is optional, consequence: any API parameter is optional by default)
# explicitly required usage ({1}) must be marked by predicate mandatoryInput (client-side contract) or mandatoryOutput (server-side conract)

ids:Parameter a owl:Class;
    rdfs:subClassOf ids:Named;
    rdfs:label "Parameter"@en ;
    rdfs:comment "Named slot of an interface operation i.e., an input, output or fault (exception)."@en;
    idsm:validation [
        idsm:forProperty ids:parameterContent;
        idsm:relationType idsm:OneToMany;
        idsm:constraint idsm:NotNull;
    ].

# Content
# reference to Content via "parameterContent" link, single cardinality per default ({1})
# explicit multiplicity marked by predicate parameterContentList ({1,n}), range of parameterContentList is Content #rdf:List
# content cardinalities along the predicate path:
#    1) input P parameterContent C {0,1}
#    3) input P parameterContentList C {0,n}
#    4) mandatoryInput P parameterContent C {1}
#    5) mandatoryInput P parameterContentList C {1,n}

ids:parameterContent a owl:ObjectProperty;
    rdfs:label "parameter content"@en ;
    rdfs:domain ids:Parameter ;
    rdfs:range ids:DigitalContent ;
    rdfs:comment "Content model of a monovalent parameter, i.e. it bounds one value at most."@en ;
    .

#ids:parameterContentList a owl:ObjectProperty;
#    rdfs:domain ids:ContentParameter;
#    rdfs:range ids:DigitalContent;
#    rdfs:label "parameter content list"@en;
#    rdfs:comment "Content model of a multivalent parameter, i.e. it may bind multiple corresponding values."@en ;
#    .

