@prefix rdf:   <http://www.w3.org/1999/02/22-rdf-syntax-ns#> .
@prefix owl: <http://www.w3.org/2002/07/owl#> .
@prefix rdfs: <http://www.w3.org/2000/01/rdf-schema#> .
@prefix xsd: <http://www.w3.org/2001/XMLSchema#> .
@prefix dcat: <http://www.w3.org/ns/dcat#> .
@prefix ids: <https://w3id.org/idsa/core/> .
@prefix idsm: <https://w3id.org/idsa/metamodel/> .

# Classes
# -------

ids:Catalog
    rdfs:subClassOf dcat:Catalog;
    a owl:Class;
    idsm:abstract true;
    rdfs:label "Catalog"@en ;
    rdfs:comment "Class that represents (distributable) Catalogs."@en ;
    .

ids:ResourceCatalog
    rdfs:subClassOf ids:Catalog;
    a owl:Class;
    rdfs:label "Resource Catalog"@en ;
    rdfs:comment "Class that aggregates Resources which, as a whole, form a (distributable) Catalog."@en ;
    idsm:validation [
        idsm:forProperty ids:requestedResource;
        idsm:relationType idsm:OneToMany;
    ];
    idsm:validation [
        idsm:forProperty ids:offeredResource;
        idsm:relationType idsm:OneToMany;
    ];
.

ids:ParticipantCatalog
    rdfs:subClassOf ids:Catalog;
    a owl:Class;
    rdfs:label "Participant Catalog"@en ;
    rdfs:comment "Class that aggregates Participants which, as a whole, from a (distributable) Catalog."@en ;
    idsm:validation [
        idsm:forProperty ids:member;
        idsm:relationType idsm:OneToMany;
    ];
.

ids:ConnectorCatalog
    rdfs:subClassOf ids:Catalog;
    a owl:Class;
    rdfs:label "Connector Catalog"@en ;
    rdfs:comment "Class that aggregates Connectors which, as a whole, from a (distributable) Catalog."@en ;
    idsm:validation [
        idsm:forProperty ids:listedConnector;
        idsm:relationType idsm:OneToMany;
    ];
.

# Properties
# ----------

ids:offeredResource a owl:ObjectProperty;
    rdfs:subPropertyOf dcat:dataset;
    rdfs:domain ids:ResourceCatalog;
    rdfs:range ids:Resource;
    rdfs:label "offered resource"@en;
    rdfs:comment "A Resource that is part of a resource catalog, indicating an offering (of, e.g., data)."@en.

ids:requestedResource a owl:ObjectProperty;
    rdfs:subPropertyOf dcat:dataset;
    rdfs:domain ids:ResourceCatalog;
    rdfs:range ids:Resource;
    rdfs:label "requested resource"@en;
    rdfs:comment "A Resource that is part of a resource catalog, indicating a request (of, e.g., data, software,...)."@en.

ids:member a owl:ObjectProperty;
    rdfs:subPropertyOf dcat:dataset;
    rdfs:domain ids:ParticipantCatalog;
    rdfs:range ids:Participant;
    rdfs:label "member"@en;
    rdfs:comment "A Participant, that is part of a participant catalog."@en.

ids:listedConnector a owl:ObjectProperty;
    rdfs:subPropertyOf dcat:dataset;
    rdfs:domain ids:ConnectorCatalog;
    rdfs:range ids:Connector;
    rdfs:label "listed Connector"@en;
    rdfs:comment "A Connector, that is part of a Connector catalog."@en;
.

