@prefix owl: <http://www.w3.org/2002/07/owl#> .
@prefix rdf:   <http://www.w3.org/1999/02/22-rdf-syntax-ns#> .
@prefix rdfs: <http://www.w3.org/2000/01/rdf-schema#> .
@prefix xsd: <http://www.w3.org/2001/XMLSchema#> .
@prefix dct: <http://purl.org/dc/terms/> .
@prefix ids: <https://w3id.org/idsa/core/> .
@prefix idsm: <https://w3id.org/idsa/metamodel/> .

# Classes
# -------

# Basic Message Types: Request, Response, Notification
# May be used direcoty for non-core IDS scenarios. 
# -----------------------------------------------------

ids:RequestMessage a owl:Class;
    rdfs:subClassOf ids:Message ;
    rdfs:label "Request Message"@en ;
    rdfs:comment "Client-generated message initiating a communication, motivated by a certain reason and with an answer expected."@en.

ids:ResponseMessage a owl:Class;
    rdfs:subClassOf ids:Message ;
    rdfs:label "Response Message"@en ;
    rdfs:comment "Response messages hold information about the reaction of a recipient to a formerly sent command or event. They must be correlated to this message."@en;
    idsm:validation [
        idsm:forProperty ids:correlationMessage;
        idsm:constraint idsm:NotNull;
    ].

ids:NotificationMessage a owl:Class ;
    rdfs:subClassOf ids:Message ;
    rdfs:label "Notification Message"@en ;
    rdfs:comment "Event messages are informative and no response is expected by the sender."@en.


# Core IDS Messages
# -----------------


ids:CommandMessage a owl:Class;
    rdfs:subClassOf ids:RequestMessage ;
    idsm:abstract true;
    rdfs:label "Command Message"@en ;
    rdfs:comment "Command messages are usually sent when a response is expected by the sender. Changes state on the recipient side. Therefore, commands are not 'safe' in the sense of REST."@en.

ids:ResultMessage a owl:Class;
    rdfs:subClassOf ids:ResponseMessage ;
    rdfs:label "Result Message"@en ;
    rdfs:comment "Result messages are intended to annotate the results of a query command. "@en.

ids:RejectionMessage a owl:Class;
    rdfs:subClassOf ids:ResponseMessage ;
    rdfs:label "Rejection Message"@en ;
    rdfs:comment "Rejection messages are specialized response messages that notify the sender of a message that processing of this message has failed."@en.

ids:RejectionReason a owl:Class;
    rdfs:label "RejectionReason"@en ;
    rdfs:comment "Class of reasons that might lead to issuing a Rejection message."@en.

ids:rejectionReason a owl:ObjectProperty;
    rdfs:domain ids:RejectionMessage;
    rdfs:range ids:RejectionReason;
    rdfs:label "rejectionReason"@en;
    rdfs:comment "Specifies the reason of the rejection."@en.

# Self-Description
# -----------------

ids:DescriptionRequestMessage a owl:Class;
    rdfs:subClassOf ids:RequestMessage ;
    rdfs:label "Description Request Message"@en ;
    rdfs:comment "Message requesting metadata. If no URI is supplied via the ids:requestedElement field, this messages is treated like a self-description request and the recipient should return its self-description via an ids:DescriptionResponseMessage. However, if a URI is supplied, the Connector should either return metadata about the requested element via an ids:DescriptionResponseMessage, or send an ids:RejectionMessage, e.g. because the element was not found." @en.

ids:DescriptionResponseMessage a owl:Class ;
    rdfs:subClassOf ids:ResponseMessage ;
    rdfs:label "Description Response Message"@en ;
    rdfs:comment "Message containing the metadata, which a Connector previously requested via the ids:DescriptionRequestMessage, in its payload."@en.

ids:requestedElement a owl:DatatypeProperty;
    rdfs:label "requested Element"@en;
    rdfs:comment "The element whose metadata is requested. "@en;
    rdfs:domain ids:DescriptionRequestMessage ;
    rdfs:range xsd:anyURI ;
.

# Connector-related Messages
# --------------------------

ids:ConnectorNotificationMessage a owl:Class;
    rdfs:subClassOf ids:NotificationMessage ;
    idsm:abstract true ;
    rdfs:label "Connector Notification Message"@en ;
    rdfs:comment "Superclass of all messages, indicating a change of a connector's conditions."@en;
    idsm:validation [
        idsm:forProperty ids:affectedConnector;
        idsm:constraint idsm:NotNull;
    ].

ids:ConnectorAvailableMessage a owl:Class;
    rdfs:subClassOf ids:ConnectorNotificationMessage ;
    rdfs:label "Connector Available Message"@en ;
    rdfs:comment "Event notifying the recipient(s) about the availability of a new connector. The payload of the message must contain the new connector's self-description."@en.

ids:ConnectorUnavailableMessage a owl:Class;
    rdfs:subClassOf ids:ConnectorNotificationMessage ;
    rdfs:label "Connector Unavailable Message"@en ;
    rdfs:comment "Event notifying the recipient(s) that a connector will be unavailable and never be available again."@en.

ids:ConnectorInactiveMessage a owl:Class;
    rdfs:subClassOf ids:ConnectorNotificationMessage ;
    rdfs:label "Connector Inactive Message"@en ;
    rdfs:comment "Event notifying the recipient(s) that a connector will be inactive and most likely be available again in the future."@en.

ids:ConnectorUpdateMessage a owl:Class;
    rdfs:subClassOf ids:ConnectorNotificationMessage ;
    rdfs:label "Connector Update Message"@en ;
    rdfs:comment "Event notifying the recipient(s) about a connector's configuration change. The payload of the message must contain the updated connector's self-description."@en.

ids:ConnectorCertificateGrantedMessage a owl:Class;
	rdfs:subClassOf ids:ConnectorNotificationMessage ;
	rdfs:label "Connector Certificate Granted Message"@en ;
	rdfs:comment "Whenever a Connector has been successfully certified by the Certification Body, the Identity Provider can use this message to notify Infrastructure Components."@en.

ids:ConnectorCertificateRevokedMessage a owl:Class;
	rdfs:subClassOf ids:ConnectorNotificationMessage ;
	rdfs:label "Connector Certificate Revoked Message"@en ;
	rdfs:comment "Indicates that a (previously certified) Connector is no more certified. This could happen, for instance, if the Certification Body revokes a granted certificate or if the certificate just expires."@en.

ids:affectedConnector a owl:ObjectProperty;
    idsm:referenceByUri true;
    rdfs:label "affected Connector"@en;
    rdfs:domain ids:ConnectorNotificationMessage;
    rdfs:range ids:Connector;
    rdfs:comment "References the connector that is affected by the runtime condition change."@en.

# Participant-related Messages
# ----------------------------
ids:ParticipantNotificationMessage a owl:Class;
    rdfs:subClassOf ids:NotificationMessage ;
    idsm:abstract true ;
    rdfs:label "Participant Notification Message"@en ;
    rdfs:comment "Superclass of all messages, indicating a change of a particpants's conditions."@en;
    idsm:validation [
        idsm:forProperty ids:affectedParticipant;
        idsm:constraint idsm:NotNull;
    ].
    

ids:ParticipantAvailableMessage a owl:Class;
    rdfs:subClassOf ids:ParticipantNotificationMessage ;
    rdfs:label "Participant Available Message"@en ;
    rdfs:comment "Event notifying the recipient(s) about the availability of a new participant. The payload of the message must contain the new connector's self-description."@en.

ids:ParticipantUnavailableMessage a owl:Class;
    rdfs:subClassOf ids:ParticipantNotificationMessage ;
    rdfs:label "Participant Unavailable Message"@en ;
    rdfs:comment "Event notifying the recipient(s) that a participant will be unavailable and never be available again."@en.

ids:ParticipantCertificateGrantedMessage a owl:Class;
    rdfs:subClassOf ids:ParticipantNotificationMessage ;
    rdfs:label "Participant Certificate Granted Message"@en ;
    rdfs:comment "Whenever a Participant has been successfully certified by the Certification Body, the Identity Provider can use this message to notify Infrastructure Components."@en.

ids:ParticipantCertificateRevokedMessage a owl:Class;
    rdfs:subClassOf ids:ParticipantNotificationMessage ;
    rdfs:label "Participant Certificate Revoked Message"@en ;
    rdfs:comment "Indicates that a (previously certified) Participant is no more certified. This could happen, for instance, if the Certification Body revokes a granted certificate or if the certificate just expires."@en.

ids:ParticipantUpdateMessage a owl:Class;
    rdfs:subClassOf ids:ParticipantNotificationMessage ;
    rdfs:label "Participant Information Changed Message"@en ;
    rdfs:comment "Event notifying the recipient(s) that information describing this Participant has changed. This event is mainly intended for information describing the Participant that is NOT a direct subject of the certification process."@en.

ids:affectedParticipant a owl:ObjectProperty;
    idsm:referenceByUri true;
    rdfs:label "affected Participant"@en;
    rdfs:domain ids:ParticipantNotificationMessage;
    rdfs:range ids:Participant;
    rdfs:comment "References the participant that is referenced in the participant-related notification messages."@en.

ids:revocationReason 
    a owl:DatatypeProperty;
    rdfs:label "Revocation Reason"@en;
    rdfs:domain [ owl:unionOf (
            ids:ConnectorCertificateRevokedMessage
            ids:ParticipantCertificateRevokedMessage
            )
        ];
    rdfs:range xsd:string;
    rdfs:comment "Plain Text containing the reason for revoking an existing certificate of either a connector or participant."@en.

# Query related Messages
# -----------------------

ids:QueryMessage a owl:Class ;
    rdfs:subClassOf ids:RequestMessage ;
    rdfs:label "Query Message"@en ;
    rdfs:comment "Query message intended to be consumed by a component."@en.

ids:QueryLanguage a owl:Class;
    rdfs:label "QueryLanguage"@en ;
    rdfs:comment "Class of query languages in which query strings may be formalized."@en.

ids:QueryScope a owl:Class;
    rdfs:label "Query Scope"@en ;
    rdfs:comment "Class of scopes that may limit the space of query results, e.g. ALL, ACTIVE_ONLY."@en.

ids:QueryTarget a owl:Class;
    rdfs:label "Query Target"@en ;
    rdfs:comment "Class of recipients of a query message, e.g. BROKER, APPSTORE, ANY."@en.

ids:queryLanguage a owl:ObjectProperty;
    rdfs:domain ids:QueryMessage;
    rdfs:range ids:QueryLanguage;
    rdfs:label "queryLanguage"@en;
    rdfs:comment "This property specifies the language of the query."@en.

ids:queryScope a owl:ObjectProperty;
    rdfs:label "queryScope"@en;
    rdfs:domain ids:QueryMessage;
    rdfs:range ids:QueryScope;
    rdfs:comment "Refers to the scope property of a query message, see ids:QueryScope."@en.

ids:recipientScope a owl:ObjectProperty;
    rdfs:label "recipient scope"@en;
    rdfs:domain ids:QueryMessage;
    rdfs:range ids:QueryTarget;
    rdfs:comment "Refers to the target property of a query message, see ids:QueryTarget."@en.


# Contract Negotiation
# --------------------

ids:ContractRequestMessage a owl:Class ;
    rdfs:subClassOf ids:RequestMessage ;
    rdfs:label "Contract Request Message"@en;
    rdfs:comment "Message containing a suggested content contract (as offered by the data consumer to the data provider) in the associated payload (which is an instance of ContractRequest)."@en ;
    .

ids:ContractResponseMessage a owl:Class ;
    rdfs:subClassOf ids:ResponseMessage ;
    rdfs:label "Contract Response Message"@en;
    rdfs:comment "Message containing a response to a contract request (of a data consumer) in form of a counter-proposal of a contract in the associated payload (which is an instance of ContractOffcer). "@en ;
    .
    
ids:ContractOfferMessage a owl:Class ;
    rdfs:subClassOf ids:NotificationMessage ;
    rdfs:label "Contract Offer Message"@en;
    rdfs:comment "Message containing a offered content contract (as offered by a data provider to the data consumer) in the associated payload (which is an instance of ContractOffer). In contrast to the ids:ContractResponseMessage, the ids:ContractOfferMessage is not related to a previous contract "@en.


ids:ContractAgreementMessage a owl:Class ;
    rdfs:subClassOf ids:ResponseMessage;
    rdfs:label "Contract Agreement Message"@en;
    rdfs:comment "Message containing a contract with resource access modalities on which two parties have agreed."@en;
    .

ids:ContractRejectionMessage a owl:Class ;
    rdfs:subClassOf ids:RejectionMessage;
    rdfs:label "Contract Rejection Message"@en;
    rdfs:comment "Message indicating rejection of a contract."@en.

ids:ContractSupplementMessage a owl:Class ;
    rdfs:subClassOf ids:NotificationMessage ;
    rdfs:label "Contract Supplement Message"@en;
    rdfs:comment "Message containing supplemental information to access resources of a contract (e.g. resource access tokens)."@en.

ids:contractRejectionReason a owl:DatatypeProperty;
    rdfs:label "Contract Rejection Reason"@en ;
    rdfs:domain ids:ContractRejectionMessage;
    rdfs:range xsd:string;
    rdfs:comment "Human-readable text describing the reason for contract rejection."@en.

ids:agreedContract a owl:ObjectProperty;
    rdfs:label "approved Contract"@en;
    rdfs:domain ids:ContractAgreementMessage;
    rdfs:range ids:ContractAgreement;
    rdfs:comment "References the Contract Agreement of two parties."@en.


# Security-related Messages
# -------------------------

ids:AccessTokenRequestMessage a owl:Class ;
    rdfs:subClassOf ids:RequestMessage ;
    rdfs:label "AccessToken Request Message"@en;
    rdfs:comment "Message requesting an access token. This is intended for point-to-point communication with, e.g., Brokers."@en.

ids:AccessTokenResponseMessage a owl:Class ;
    rdfs:subClassOf ids:ResponseMessage ;
    rdfs:label "Access Token Response"@en;
    rdfs:comment "Response to an access token request, intended for point-to-point communication."@en.


# Resource related messages
# -------------------------

ids:ResourceNotificationMessage a owl:Class;
    rdfs:subClassOf ids:NotificationMessage ;
    idsm:abstract true ;
    rdfs:label "Resource Notification Message"@en ;
    rdfs:comment "Superclass of all messages, indicating a change of a resource."@en;
	idsm:validation [
        idsm:forProperty ids:affectedResource;
        idsm:constraint idsm:NotNull;
    ].

ids:ResourceAvailableMessage a owl:Class ;
    rdfs:subClassOf ids:ResourceNotificationMessage ;
    rdfs:label "Resource Available Message"@en;
    rdfs:comment "Message indicating that a specific resource is available."@en.

ids:ResourceUpdateMessage a owl:Class ;
    rdfs:subClassOf ids:ResourceNotificationMessage ;
    rdfs:label "Resource Update Message"@en;
    rdfs:comment "Message indicating an update of a specific resource."@en.

ids:ResourceUnavailableMessage a owl:Class ;
    rdfs:subClassOf ids:ResourceNotificationMessage ;
    rdfs:label "Resource Unavailable Message"@en;
    rdfs:comment "Message indicating that a specific resource is unavailable."@en.

ids:affectedResource rdf:type owl:ObjectProperty ;
    rdfs:domain ids:ResourceNotificationMessage;
    rdfs:range ids:Resource ;
    rdfs:label "affected Resource"@en ;
    rdfs:comment "The affected resource that is referenced in the resource-related notification messages. "@en.


ids:InvokeOperationMessage a owl:Class ;
    rdfs:subClassOf ids:RequestMessage ;
    rdfs:label "Invoke Operation Message"@en;
    rdfs:comment "Message requesting the recipient to invoke a specific operation."@en;
    idsm:validation [
        idsm:forProperty ids:operationReference;
        idsm:constraint idsm:NotNull;
    ];
    idsm:validation [
        idsm:forProperty ids:operationParameterization;
        idsm:constraint idsm:NotNull;
    ].

ids:operationReference rdf:type owl:DatatypeProperty ;
    idsm:referenceByUri true;
    rdfs:domain ids:InvokeOperationMessage ;
    rdfs:range ids:Operation ;
    rdfs:label "Operation Reference"@en ;
    rdfs:comment "References the operation to be invoked on the recipient's side by an URI."@en.

ids:operationParameterization rdf:type owl:DatatypeProperty ;
    rdfs:domain ids:InvokeOperationMessage ;
    rdfs:range ids:ParameterAssignment ;
    rdfs:label "Operation Parameterization"@en ;
    rdfs:comment "Parameter assignment of the invoked operation's input parameters."@en.

ids:RequestInProcessMessage a owl:Class ;
    rdfs:subClassOf ids:NotificationMessage;
    rdfs:label "Request In Process Message"@en;
    rdfs:comment "Notification that a request has been accepted and is being processed."@en;
    idsm:validation [
        idsm:forProperty ids:correlationMessage;
        idsm:constraint idsm:NotNull;
    ].

ids:MessageProcessedNotificationMessage a owl:Class ;
    rdfs:subClassOf ids:NotificationMessage;
    rdfs:label "Message Processed Notification Message"@en;
    rdfs:comment "Notification that a message has been successfully processed (i.e. not ignored or rejected)."@en;
    idsm:validation [
        idsm:forProperty ids:correlationMessage;
        idsm:constraint idsm:NotNull;
    ].

ids:OperationResultMessage  a owl:Class ;
    rdfs:subClassOf ids:ResponseMessage;
    rdfs:label "Operation Result Message"@en;
    rdfs:comment "Message indicating that the result of a former InvokeOperation message is available. May transfer the result data in its associated payload section."@en.


# Artifact-related Messages
# -------------------------

ids:ArtifactRequestMessage a owl:Class ;
    rdfs:subClassOf ids:RequestMessage ;
    rdfs:label "Artifact Request Message"@en;
    rdfs:comment "Message asking for retrieving the specified Artifact as the payload of an ArtifactResponse message."@en;
    idsm:validation [
        idsm:forProperty ids:requestedArtifact;
        idsm:constraint idsm:NotNull;
    ].

ids:ArtifactResponseMessage a owl:Class ;
    rdfs:subClassOf ids:ResponseMessage;
    rdfs:label "Artifact Response Message"@en;
    rdfs:comment "Message that follows up a RetrieveArtifact Message and contains the Artifact's data in the payload section."@en.

ids:requestedArtifact rdf:type owl:ObjectProperty ;
    idsm:referenceByUri true;
    rdfs:domain ids:ArtifactRequestMessage;
    rdfs:range ids:Artifact ;
    rdfs:label "Requested Artifact"@en ;
    rdfs:comment "References an artifact in the context of a request."@en.


# ParIS Messages
# --------------

ids:ParticipantRequestMessage a owl:Class ;
    rdfs:subClassOf ids:RequestMessage ;
    rdfs:label "Participant Request Message"@en;
    rdfs:comment "Message asking for retrieving the specified Participants information as the payload of an ParticipantResponse message."@en;
    idsm:validation [
        idsm:forProperty ids:requestedParticipant;
        idsm:constraint idsm:NotNull;
    ].

ids:ParticipantResponseMessage a owl:Class ;
    rdfs:subClassOf ids:ResponseMessage;
    rdfs:label "Participant Response Message"@en;
    rdfs:comment "Message that follows up a ParticipantRequestMessage and contains the Participant's information in the payload section."@en.

ids:requestedParticipant rdf:type owl:ObjectProperty ;
    idsm:referenceByUri true;
    rdfs:domain ids:ParticipantRequestMessage;
    rdfs:range ids:Participant ;
    rdfs:label "Requested Participant"@en ;
    rdfs:comment "References a Participant in the context of a request."@en.


# Log messaging
# -------------

ids:LogMessage a owl:Class;
    rdfs:subClassOf ids:NotificationMessage ;
    rdfs:label "Log Message"@en ;
    rdfs:comment "Log Message which can be used to transfer logs e.g. to the clearing house."@en.

