@prefix owl: <http://www.w3.org/2002/07/owl#> .
@prefix rdf:   <http://www.w3.org/1999/02/22-rdf-syntax-ns#> .
@prefix rdfs: <http://www.w3.org/2000/01/rdf-schema#> .
@prefix xsd: <http://www.w3.org/2001/XMLSchema#> .
@prefix dct: <http://purl.org/dc/terms/> .
@prefix ids: <https://w3id.org/idsa/core/> .
@prefix idsm: <https://w3id.org/idsa/metamodel/> .

# Classes
# -------

# Parameter subclasses reflect the purpose of a Parameter and support
# the definition of restrictions on Operation signatures based on Parameter type

# Identification

ids:IdentifierParameter
    a owl:Class ;
    rdfs:subClassOf ids:Parameter ;
    rdfs:label "Identifier parameter"@en ;
    rdfs:comment "Parameter for conveying identifiers as defined by, e.g. an element collection (name/key). The identifier is unique and valid (in a defined context) regardless of the actual extent, ordering, and view (filtering)."@en ;
    .

ids:IndexParameter
    a owl:Class ;
    rdfs:subClassOf ids:Parameter ;
    rdfs:label "Index parameter"@en ;
    rdfs:comment "Parameter conveying the transient, positional identifier of a resource in the context of an ordered Collection. The resource index is temporarily unique and valid only with respect to the actual extent, ordering, and view (filtering) of the Collection."@en ;
    .

# Content

ids:ResourceParameter
    a owl:Class ;
    rdfs:subClassOf ids:Parameter ;
    rdfs:label "Resource parameter"@en ;
    # Top-level content linked immediately by the resource
    rdfs:comment "Parameter conveying a representation of resource's principal content, contrasted to parameters mediating arbitrary data."@en ;
    .

# Sorting

# ASC / DESC
ids:SortOrderParameter
    a owl:Class ;
    rdfs:subClassOf ids:Parameter ;
    rdfs:label "Sort order parameter"@en ;
    rdfs:comment "Parameter indicating the sort direction of an ordered Collection."@en ;
    .

# List of column identifiers
ids:SortKeyParameter
    a owl:Class ;
    rdfs:subClassOf ids:Parameter ;
    rdfs:label "Sort key parameter"@en ;
    rdfs:comment "Parameter indicating the keys underlying the sorting of an ordered Collection."@en ;
    .

# Client-defined content view - support for "content pagination"

# Signed int
ids:OffsetParameter
    a owl:Class ;
    rdfs:subClassOf ids:Parameter ;
    rdfs:label "Offset parameter"@en ;
    rdfs:comment "Parameter indicating the absolute offset (number of data elements to skip) within an ordered data Collection. Negative values are bounded at Collections's end (reverse) index."@en ;
    .

# nonNegativeInt > 0
ids:LimitParameter
    a owl:Class ;
    rdfs:subClassOf ids:Parameter ;
    rdfs:label "Limit parameter"@en ;
    rdfs:comment "Parameter indicating the number of elements retrieved or provided at once within a paginated subset (page)."@en ;
    .

# Server-defined content view, i.e. clients navigate predefined content "pages" by index or reference

# Signed int, same as offset
ids:PageIndexParameter
    a owl:Class ;
    rdfs:subClassOf ids:IndexParameter ;
    rdfs:label "Page index parameter"@en ;
    rdfs:comment "Parameter conveying the transient, positional identifier of a content page within a server-defined pagination."@en ;
    .

# Relative page reference (first/last etc.), see codes/PageReference.ttl
ids:PageReferenceParameter
    a owl:Class ;
    rdfs:subClassOf ids:Parameter ;
    rdfs:label "Page reference parameter"@en ;
    rdfs:comment "Parameter conveying a relative reference to a content page within a server-defined pagination."@en ;
    .

# Filtering - listing matching contents

# LDAP Filter, XPath/JSONPath
ids:FilterParameter
    a owl:Class ;
    rdfs:subClassOf ids:Parameter ;
    rdfs:label "Filter parameter"@en ;
    rdfs:comment "Parameter holding a filter expression (matcher) used to identify a matching selection of contents."@en ;
    .

# Selection - extracting matching content parts

# XQuery, SPARQL Construct/Select
ids:SelectorParameter
    a owl:Class ;
    rdfs:subClassOf ids:Parameter ;
    rdfs:label "Selector parameter"@en ;
    rdfs:comment "Parameter holding a selector expression used to retrieve a subset of a Resource contents."@en ;
    .

