@prefix dct: <http://purl.org/dc/terms/> .
@prefix dcat: <http://www.w3.org/ns/dcat#> .
@prefix owl: <http://www.w3.org/2002/07/owl#> .
@prefix rdf: <http://www.w3.org/1999/02/22-rdf-syntax-ns#> .
@prefix rdfs: <http://www.w3.org/2000/01/rdf-schema#> .
@prefix xsd: <http://www.w3.org/2001/XMLSchema#> .
@prefix ids: <https://w3id.org/idsa/core/> .
@prefix idsm: <https://w3id.org/idsa/metamodel/> .

# Classes
# -------

ids:Artifact
    a owl:Class;
    rdfs:subClassOf ids:RepresentationInstance; # dcat:Distribution partial subclass of dcat:Distribution w.r.t materialization aspects
    rdfs:label "Artifact"@en ;
    rdfs:comment "Instance of a Representation materialized at a partiuclar version and point in time. Possesses characteristics like file name, size, creation date etc."@en ;
    owl:disjointWith ids:Value .

# Replaced by ids:Value
#ids:InlineArtifact
#    a owl:Class;
#    rdfs:subClassOf ids:Artifact ;
#    rdfs:label "Inline Artifact"@en ;
#    rdfs:comment "Artifact which content is maintained along with the description and is available for immediate retrieval."@en.

# Obsolated by Artifact exposed by an endpoint
#ids:RemoteArtifact
#    a owl:Class;
#    rdfs:subClassOf ids:Artifact ;
#    rdfs:label "Remote Artifact"@en ;
#    rdfs:comment "Artifact which content is maintained separately from the description."@en ;
#    owl:disjointWith ids:InlineArtifact .

# Properties
# ----------

ids:byteSize
    a owl:DatatypeProperty;
    rdfs:subPropertyOf dcat:byteSize ;
    rdfs:label "byte size"@en ;
    rdfs:comment "Size of the Artifact in bytes."@en ;
    rdfs:domain ids:Artifact ;
    rdfs:range xsd:nonNegativeInteger .

ids:fileName
    a owl:DatatypeProperty;
    rdfs:label "file name"@en ;
    rdfs:comment "Name of the Artifcat file."@en ;
    rdfs:domain ids:Artifact ;
    rdfs:range xsd:string .

ids:creationDate
    a owl:DatatypeProperty;
    rdfs:subPropertyOf dct:created ;
    rdfs:label "creation date"@en ;
    rdfs:comment "Date (as xsd:dateTimeStamp) when the artifact was created, i.e. persisted."@en ;
    rdfs:domain ids:Artifact ;
    rdfs:range xsd:dateTimeStamp .

ids:artifactParameterization
    a owl:ObjectProperty;
    rdfs:domain ids:Artifact ;
    rdfs:range ids:ParameterAssignment;
    rdfs:label "artifact parameterization"@en;
    rdfs:comment "Reference to a parameter assignment that describes how an artifact has been created."@en.

# replaced by ids:Value
#ids:literalValue
#    a owl:DatatypeProperty;
#    rdfs:domain ids:InlineArtifact ;
#    rdfs:range xsd:string ;
#    rdfs:label "literal value"@en ;
#    rdfs:comment "Literal value of the Artifcat."@en .

#ids:base64Value
#    a owl:DatatypeProperty;
#    rdfs:domain ids:InlineArtifact ;
#    rdfs:range xsd:base64Binary ;
#    rdfs:label "Base64-encoded value"@en ;
#    rdfs:comment "Base64-encoded value of the Artifcat."@en .

ids:checkSum
    a owl:DatatypeProperty;# spdx:checksum has range spdx:Checksum; https://spdx.org/rdf/terms/#checksum
    rdfs:domain ids:Artifact ;
    rdfs:range xsd:string ;
    rdfs:label "checksum"@en ;
    rdfs:comment "Checksum of the artifact"@en .

# Media artifacts
ids:duration
    a owl:DatatypeProperty;
    rdfs:domain ids:Artifact ;
    rdfs:range xsd:decimal ;# duration in seconds
    rdfs:label "duration"@en ;
    rdfs:comment "Duration of the media resource in seconds."@en .

# with integration of endpoints for direct artifact download, download url and access url may be obsolete
#ids:downloadUrl # since domain of dcat:downloadURL is rdfs:Resource not applicable as super-property, URL is not a resource
#    a owl:DatatypeProperty;
#    rdfs:domain ids:RemoteArtifact ;
#    rdfs:range xsd:anyURI ;
#    rdfs:label "Download URL"@en ;
#    rdfs:comment "Resolvable web address providing for the direct download of Artifact content."@en .

#ids:accessUrl # since domain of dcat:accessURL is rdfs:Resource not applicable as super-property, URL is not a resource
#    a owl:DatatypeProperty;
#    rdfs:domain ids:RemoteArtifact ;
#    rdfs:range xsd:anyURI ;
#    rdfs:label "Access URL"@en ;
#    rdfs:comment "Resolvable web address providing for an indirect access to artifact contents."@en .

# dct:issued
# idsm:constantIdentifier
# dct:title
# dct:description
# dct:licence
# dct:rights

