@prefix rdf:   <http://www.w3.org/1999/02/22-rdf-syntax-ns#> .
@prefix owl: <http://www.w3.org/2002/07/owl#> .
@prefix rdfs: <http://www.w3.org/2000/01/rdf-schema#> .
@prefix dct: <http://purl.org/dc/terms/> .
@prefix dcat: <http://www.w3.org/ns/dcat#> .
@prefix ids: <https://w3id.org/idsa/core/> .
@prefix idsm: <https://w3id.org/idsa/metamodel/> .
@prefix xsd: <http://www.w3.org/2001/XMLSchema#> .

# Classes
# -------

ids:DigitalContent
    a owl:Class;    
    rdfs:subClassOf ids:Described, dcat:Dataset;
    rdfs:label "Digital content"@en ;
    rdfs:comment "Digital content of a particular type providing hints on its usage, e.g. listening to an Audio, navigating a Structure or accessing a List by an index."@en ;
    idsm:validation [
        idsm:forProperty ids:contentPart;
        idsm:relationType idsm:OneToMany;
    ];
    idsm:validation [
        idsm:forProperty ids:spatialCoverage;
        idsm:relationType idsm:OneToMany;
    ];
    idsm:validation [
        idsm:forProperty ids:temporalCoverage;
        idsm:relationType idsm:OneToMany;
    ];
    idsm:validation [
        idsm:forProperty ids:language;
        idsm:relationType idsm:OneToMany;
    ];
    idsm:validation [
        idsm:forProperty ids:theme;
        idsm:relationType idsm:OneToMany;
    ];
    idsm:validation [
        idsm:forProperty ids:keyword;
        idsm:relationType idsm:OneToMany;
    ];
    idsm:validation [
        idsm:forProperty ids:contentRefinement;
        idsm:relationType idsm:OneToMany;
    ];
    idsm:validation [
        idsm:forProperty ids:representation;
        idsm:relationType idsm:OneToMany;
    ];
    idsm:abstract true ;
    rdfs:seeAlso
        <https://en.wikipedia.org/wiki/Digital_content> ,
        <http://www.ontodm.com/doku.php?id=ontodt> ,
        # <https://schema.org/DataType> ,
        # <https://schema.org/additionalType> ,
        <http://schema.org/DataType> ,
        <http://schema.org/additionalType> ,
        <https://github.com/twosixlabs/icas-ontology/blob/master/ontology/mime.ttl> ,
        <http://www.ddialliance.org/Specification/DDI-CV/GeneralDataFormat_2.0.html>. # GeneralDataFormat, formerly KindOfDataFormat

# Properties
# general "content" properties here, otherwise with concrete subclasses
# ------------

ids:contentType
    a owl:ObjectProperty;
    rdfs:domain ids:DigitalContent;
    rdfs:range ids:ContentType;
    rdfs:label "content type"@en;
    rdfs:comment "Detailed type, genre or interpretation of the Digital Content."@en.

ids:contentPart
    a owl:ObjectProperty;
    rdfs:subPropertyOf dct:hasPart;
    rdfs:label "content part"@en;
    rdfs:domain ids:DigitalContent;
    rdfs:range ids:DigitalContent;
    rdfs:comment "Reference to a Digital Content (physically or logically) included, definition of part-whole hierarchies."@en .

ids:representation
    a owl:ObjectProperty;
    #rdfs:subPropertyOf dcat:distribution ; # Links to non-materialized part of Distribution
    rdfs:label "representation"@en;
    rdfs:domain ids:DigitalContent;
    rdfs:range ids:Representation;
    rdfs:comment "Representation of the content."@en.

ids:defaultRepresentation
    a owl:ObjectProperty;
    rdfs:subPropertyOf ids:representation ;
    rdfs:label "Default representation"@en;
    rdfs:domain ids:DigitalContent;
    rdfs:range ids:Representation;
    rdfs:comment "Default representation of the content."@en.

ids:language
    a owl:ObjectProperty;
    rdfs:subPropertyOf dct:language;
    rdfs:domain ids:DigitalContent;
    rdfs:range ids:Language; # does not fit the defined range of dct:language - dct:LinguisticSystem !
    rdfs:label "language"@en;
    rdfs:comment "Natural language(s) used within the content."@en.

ids:theme # ... "topic" / "subject" ?
    a owl:ObjectProperty;
    rdfs:subPropertyOf dcat:theme; # is a sub-property of dct:subject, comparable to qb:concept (?)
    idsm:referenceByUri true ;
    rdfs:label "theme"@en;
    rdfs:domain ids:DigitalContent;
    rdfs:range ids:Concept; # former "ContentCategory", skos:Concepts organized in a skos:ConceptScheme
    rdfs:comment "Abstract or concrete concept related to or referred by the content."@en.


ids:keyword
    a owl:DatatypeProperty;
    rdfs:subPropertyOf dcat:keyword;
    rdfs:label "keyword"@en;
    rdfs:domain ids:DigitalContent;
    rdfs:range xsd:string;
    rdfs:comment "Controlled keywords that describe the nature, purpose, or use of the content."@en.

ids:temporalCoverage
    a owl:ObjectProperty;
    rdfs:subPropertyOf dct:temporal;
    rdfs:label "temporal coverage"@en;
    rdfs:domain ids:DigitalContent;
    rdfs:range ids:TemporalEntity;
    rdfs:comment "Temporal period or instance covered by the content."@en.

ids:spatialCoverage
    a owl:ObjectProperty;
    rdfs:subPropertyOf dct:spatial;
    rdfs:label "spatial coverage"@en;
    rdfs:domain ids:DigitalContent;
    rdfs:range ids:SpatialEntity;
    rdfs:comment "Named spatial entity covered by the Resource."@en.

ids:accrualPeriodicity # consider irregular updates as well
    a owl:DatatypeProperty;
    # rdfs:subPropertyOf dct:accrualPeriodicity - not applicable, since range is a dct:Frequency
    rdfs:label "Accrual periodicity"@en;
    rdfs:comment "The regular period with which items are added to a collection."@en ;
    rdfs:domain ids:DigitalContent;
    rdfs:range xsd:duration;
    .

ids:contentStandard
    idsm:referenceByUri true;
    a owl:ObjectProperty ;
    rdfs:subPropertyOf dct:conformsTo ;
    rdfs:domain ids:DigitalContent ;
    rdfs:range ids:Standard;
    rdfs:label "content standard"@en;
    rdfs:comment "Standards document defining the given Digital Content. The content is assumed to conform to that Standard."@en.

ids:created
    a owl:DatatypeProperty ;
    rdfs:subPropertyOf dct:issued;
    rdfs:domain [ rdf:type owl:Class ;
                owl:unionOf ( ids:DigitalContent ids:Representation)
              ] ;
    rdfs:range xsd:dateTimeStamp ;
    rdfs:label "created"@en;
    rdfs:seeAlso <http://purl.org/dc/terms/created> ;
    rdfs:comment "The date of the creation of the Digital Content. In contrast to the ids:temporalCoverage, creation dates of ids:Representation, ids:Artifacts or any other form of meta-data, this property describes the creation date of referenced Digital Content itself."@en.

ids:modified
    a owl:DatatypeProperty;
    rdfs:subPropertyOf dct:modified;
    rdfs:domain [ rdf:type owl:Class ;
                owl:unionOf ( ids:DigitalContent ids:Representation)
              ] ;
    rdfs:range xsd:dateTimeStamp;
    rdfs:label "modified"@en;
    rdfs:seeAlso <http://purl.org/dc/terms/modified> ;
    rdfs:comment "The date/time this Digital Content has been changed the last time. Only one 'modified' attribute is usually needed."@en.
