@prefix rdf:   <http://www.w3.org/1999/02/22-rdf-syntax-ns#> .
@prefix owl: <http://www.w3.org/2002/07/owl#> .
@prefix rdfs: <http://www.w3.org/2000/01/rdf-schema#> .
@prefix xsd: <http://www.w3.org/2001/XMLSchema#> .
@prefix dcat: <http://www.w3.org/ns/dcat#> .
@prefix ids: <https://w3id.org/idsa/core/> .
@prefix idsm: <https://w3id.org/idsa/metamodel/> .

# Classes
# -------

ids:Catalog
    rdfs:subClassOf dcat:Catalog;
    a owl:Class;
    rdfs:label "Catalog"@en ;
    rdfs:comment "Class that aggregates Resources which, as a whole, form a (distributable) Catalog."@en ;
    idsm:validation [
        idsm:forProperty ids:request;
        idsm:relationType idsm:OneToMany;
    ];
    idsm:validation [
        idsm:forProperty ids:offer;
        idsm:relationType idsm:OneToMany;
    ].

# Properties
# ----------

ids:offer a owl:ObjectProperty;
    rdfs:domain ids:Catalog;
    rdfs:range ids:Resource;
    rdfs:label "offer"@en;
    rdfs:comment "A Resource that is part of a Connector, indicating a offering (of, e.g., data)."@en.

ids:request a owl:ObjectProperty;
    rdfs:domain ids:Catalog;
    rdfs:range ids:Resource;
    rdfs:label "request"@en;
    rdfs:comment "A Resource that is part of a Connector, indicating a request (of, e.g., data, software,...)."@en.

