@prefix owl: <http://www.w3.org/2002/07/owl#> .
@prefix rdfs: <http://www.w3.org/2000/01/rdf-schema#> .
@prefix dct: <http://purl.org/dc/terms/> .
@prefix prov: <http://www.w3.org/ns/prov#> .
@prefix xsd: <http://www.w3.org/2001/XMLSchema#> .
@prefix rdf: <http://www.w3.org/1999/02/22-rdf-syntax-ns#> .
@prefix ids: <https://w3id.org/idsa/core/> .
@prefix idsm: <https://w3id.org/idsa/metamodel/> .

# Classes
# -------

ids:Activity rdfs:subClassOf prov:Activity;
    a owl:Class;
    idsm:abstract true;
    rdfs:label "Activity"@en ;
    rdfs:comment "Something that occurs over a period of time and acts upon or with entities."@en;
    rdfs:seeAlso <http://www.ddialliance.org/Specification/DDI-CV/LifecycleEventType_1.0.html>;# DDI Lifecycle Event Type
    idsm:validation [
        idsm:forProperty ids:startedBy;
        idsm:constraint idsm:NotNull;
    ];
    idsm:validation [
        idsm:forProperty ids:startedAt;
        idsm:constraint idsm:NotNull;
    ];
    idsm:validation [
        idsm:forProperty ids:activityDescription;
        idsm:relationType idsm:OneToMany;
    ].

ids:CreationActivity rdfs:subClassOf ids:Activity;
    a owl:Class;
    rdfs:label "CreationActivity"@en ;
    rdfs:comment "Activity with the goal to generate or produce an entity."@en.

ids:RemovalActivity rdfs:subClassOf ids:Activity;
    a owl:Class;
    rdfs:label "RemovalActivity"@en ;
    rdfs:comment "Activity with the goal to decommission an entity so that it can never be used anymore."@en.

ids:ProvisioningActivity rdfs:subClassOf ids:Activity;
    a owl:Class;
    rdfs:label "ProvisioningActivity"@en ;
    rdfs:comment "Activity with the goal to bring an entity into an operational state."@en.

ids:ShutdownActivity rdfs:subClassOf ids:Activity;
    a owl:Class;
    rdfs:label "ShutdownActivity"@en ;
    rdfs:comment "Activity with the goal to make an entity unoperational, while retaining it and make it operational again at a later point in time."@en.

ids:PublicationActivity rdfs:subClassOf ids:Activity;
    a owl:Class;
    rdfs:label "PublicationActivity"@en ;
    rdfs:comment "Activity with the goal to make available an entity for public or restricted access."@en.

ids:WithdrawActivity rdfs:subClassOf ids:Activity;
    a owl:Class;
    rdfs:label "WithdrawActivity"@en ;
    rdfs:comment "Activity with the goal to withdraw public or restrict availability of an entity."@en.

ids:SuspensionActivity rdfs:subClassOf ids:Activity;
    a owl:Class;
    rdfs:label "SuspensionActivity"@en ;
    rdfs:comment "Activity with the goal to temporarily suspend operation of an entity."@en.

ids:ResumptionActivity rdfs:subClassOf ids:Activity;
    a owl:Class;
    rdfs:label "ResumptionActivity"@en ;
    rdfs:comment "Activity with the goal to resume operation of a temporarily suspended entity."@en.

ids:ModificationActivity rdfs:subClassOf ids:Activity;
    a owl:Class;
    rdfs:label "ModificationActivity"@en ;
    rdfs:comment "Activity that sustainably modifies the managed entity, resulting in a new version."@en.

# Properties
# ----------

ids:activityDescription rdfs:subPropertyOf dct:description;
    a owl:DatatypeProperty;
    rdfs:domain ids:Activity;
    rdfs:range xsd:string;
    rdfs:label "activityDescription"@en;
    rdfs:comment "Freetext description of what has been performed by the Activity."@en.

ids:startedBy rdfs:subPropertyOf prov:wasStartedBy;
    a owl:ObjectProperty;
    rdfs:domain ids:Activity;
    rdfs:range ids:Participant;
    rdfs:label "startedBy"@en;
    rdfs:comment "The participant who started the Activity."@en.

ids:startedAt rdfs:subPropertyOf prov:startedAtTime;
    a owl:DatatypeProperty;
    rdfs:domain ids:Activity;
    rdfs:range xsd:dateTimeStamp;
    rdfs:label "startedAt"@en;
    rdfs:comment "The point in time (as xsd:dateTimeStamp) when the Activity was started."@en.

ids:endedBy rdfs:subPropertyOf prov:wasEndedBy;
    a owl:ObjectProperty;
    rdfs:domain ids:Activity;
    rdfs:range ids:Participant;
    rdfs:label "endedBy"@en;
    rdfs:comment "The participant who ended the Activity."@en.

ids:endedAt rdfs:subPropertyOf prov:endedAtTime;
    a owl:DatatypeProperty;
    rdfs:domain ids:Activity;
    rdfs:range xsd:dateTimeStamp;
    rdfs:label "endedAt"@en;
    rdfs:comment "The point in time (as xsd:dateTimeStamp) when the Activity was ended."@en.

ids:invalidated rdfs:subPropertyOf prov:invalidated;
    a owl:DatatypeProperty;
    rdfs:domain ids:ModificationActivity;
    rdfs:range ids:ManagedEntity;
    rdfs:label "originalEntity"@en;
    rdfs:comment "Managed Entity that was the source of the modification."@en.

