@prefix owl: <http://www.w3.org/2002/07/owl#> .
@prefix rdf: <http://www.w3.org/1999/02/22-rdf-syntax-ns#> .
@prefix rdfs: <http://www.w3.org/2000/01/rdf-schema#> .
@prefix xsd: <http://www.w3.org/2001/XMLSchema#> .
@prefix dct: <http://purl.org/dc/terms/> .
@prefix ids: <https://w3id.org/idsa/core/> .


# Classes
# -------

ids:EndpointBinding
    a owl:Class ;
    rdfs:label "Endpoint binding"@en ;
    rdfs:comment "Description of endpoints a App offers as (API) bindings."@en ;
.


# Properties
# -------

ids:apiSpecReference
    a owl:DatatypeProperty ;
    rdfs:domain ids:EndpointBinding ;
    rdfs:range xsd:anyURI ;
	rdfs:label "api spec reference"@en ;
    rdfs:comment "IRI reference to the api specification for the endpoints. "@en ;
.

ids:apiSpec 
    a owl:DatatypeProperty ;
    rdfs:domain ids:EndpointBinding ;
    rdfs:range xsd:string ;
	rdfs:label "api spec"@en ;
    rdfs:comment "The api specification for the endpoint binding as raw data. It is recommended to use the ids:apiSpecReference property. This property should be used, when it is not possible to refer to an api specification using IRIs."@en ;
.

ids:apiSpecVersion
    a owl:DatatypeProperty ;
    rdfs:domain ids:EndpointBinding ;
    rdfs:range xsd:string ;
	rdfs:label "api spec version"@en ;
    rdfs:comment "The version of the API specification."@en ;
.

ids:protocolType
	a owl:ObjectProperty ;
	rdfs:domain ids:EndpointBinding ;
	rdfs:range ids:ProtocolType ;
	rdfs:label "protocol type"@en ;
	rdfs:comment "The protocol of the referenced API specification. Uses a controlled list of protocol types."@en ;
.	

ids:endpointReference
	a owl:ObjectProperty ;
	rdfs:domain ids:EndpointBinding ;
	rdfs:range ids:EndpointReference ;
	rdfs:label "endpoint reference"@en ;
	rdfs:comment "Endpoint references are used to refer to subsections of API specifications. Using the ids:EndpointReference and ids:AppEndpointType classes, specific endpoints/sections of APIs can be labeled with the data app endpoint type."@en ;
.	
