@prefix owl: <http://www.w3.org/2002/07/owl#> .
@prefix rdf: <http://www.w3.org/1999/02/22-rdf-syntax-ns#> .
@prefix rdfs: <http://www.w3.org/2000/01/rdf-schema#> .
@prefix xsd: <http://www.w3.org/2001/XMLSchema#> .
@prefix dct: <http://purl.org/dc/terms/> .
@prefix ids: <https://w3id.org/idsa/core/> .


# Classes
# -------

ids:EndpointReference
    a owl:Class ;
    rdfs:label "Endpoint reference"@en ;
    rdfs:comment "Class to reference subsections of endpoint APIs. Can be used to label sections of APIs with the corresponding data app endpoint type. See ids:AppEndpointType for list of endpoint types for data apps."@en ;
.

ids:value
    a owl:DatatypeProperty ;
    rdfs:domain ids:EndpointReference ;
    rdfs:range xsd:string ;
	rdfs:label "value"@en ;
    rdfs:comment "Endpoint reference value. Sections of the APIs can be refered by e.g., JSON references."@en ;
	rdfs:seeAlso <https://swagger.io/docs/specification/using-ref/> ;
.

ids:appEndpointType
    a owl:ObjectProperty ;
    rdfs:domain ids:EndpointReference ;
    rdfs:range ids:AppEndpointType ;
    rdfs:label "App endpoint type"@en ;
    rdfs:comment "Type of an data app endpoint. Data apps have different endpoint types, e.g., for input, output or status."@en ;
.