@prefix owl: <http://www.w3.org/2002/07/owl#> .
@prefix rdf:   <http://www.w3.org/1999/02/22-rdf-syntax-ns#> .
@prefix rdfs: <http://www.w3.org/2000/01/rdf-schema#> .
@prefix xsd: <http://www.w3.org/2001/XMLSchema#> .
@prefix ids: <https://w3id.org/idsa/core/> .
@prefix dct: <http://purl.org/dc/terms/> .

ids:BusinessIdentifier
	a owl:Class;
	rdfs:label "Business Identifier"@en;
    rdfs:comment "A business identifier is a identification number used to identify a company. E.g., the Data Universal Numbering System, abbreviated as DUNS"@en;
.

ids:identifierSystem
    a            owl:DatatypeProperty ;
    rdfs:domain  ids:BusinessIdentifier ;
    rdfs:range   xsd:string ;
    rdfs:label   "identifier system"@en ;
    rdfs:comment "This property is used to define the system used as an business identifier. E.g., DUNS or SIRET."@en ;
.

ids:identifierNumber
    a            owl:DatatypeProperty ;
	rdfs:subPropertyOf dct:identifier ;
    rdfs:domain  ids:BusinessIdentifier  ;
    rdfs:range   xsd:string ;
    rdfs:label   "identifier number"@en ;
    rdfs:comment "This property is used to define the value used as an business identifier."@en ;
.
	
	