@prefix owl: <http://www.w3.org/2002/07/owl#> .
@prefix rdfs: <http://www.w3.org/2000/01/rdf-schema#> .
@prefix skos: <http://www.w3.org/2004/02/skos/core#> .
@prefix ids: <https://w3id.org/idsa/core/> .
@prefix idsm: <https://w3id.org/idsa/metamodel/> .

# Classes
# -------

ids:Role
    a owl:Class ;
    rdfs:label "Role"@en ;
    rdfs:comment "Generic notion of a role played by participant in context of the Industrial Data Space." ;
    idsm:abstract true .

ids:Applicant
    rdfs:subClassOf ids:Role ;
    rdfs:label "Applicant"@en ;
    rdfs:comment "Organization formally applying for being certified by the Certification Body."@en .

ids:BrokerServiceProvider
    rdfs:subClassOf ids:Role ;
    rdfs:label "Broker Service Provider"@en ;
    rdfs:comment "Intermediary managing a metadata repository that provides information about the Data Sources available in the Industrial Data Space; multiple Broker Service Providers may be around at the same time, maintaining references to different, domain-specific subsets of Data Endpoints."@en .

ids:CertificationAuthority
    rdfs:subClassOf ids:Role ;
    rdfs:label "Certification Authority"@en ;
    rdfs:comment "Trusted third-party entity issuing digital certificates (e.g., x509 certificates); may host services to validate certificates issued."@en .

#ids:CertificationBody
#    rdfs:subClassOf ids:Role ;
#    rdfs:label "Certification Body"@en ;
#    rdfs:comment "Governance body certifying components and entities seeking admission to the Industrial Data Space; aside from having the final word on granting or denying a certificate, it is responsible for maintaining the Certification Scheme (including its catalog of requirements), for overseeing and approval of Evaluation Facilities, and for ensuring compatibility of evaluation procedures carried out by different Evaluation Facilities."@en .

#ids:ClearingHouse
#    rdfs:subClassOf ids:Role ;
#    rdfs:label "Clearing House"@en ;
#    rdfs:comment "Intermediary providing clearing and settlement services for all financial and data exchange transactions within the Industrial Data Space."@en .

ids:DataConsumer
    rdfs:subClassOf ids:Role;
    rdfs:label "Data Consumer"@en ;
    rdfs:comment "Core participant in the Industrial Data Space requesting and using data provided by a Data Provider."@en .

ids:DataSovereign
    rdfs:subClassOf ids:Role;
    rdfs:label "Data Sovereign"@en ;# ids:Agent -> will become an contract assigner
    skos:altLabel "Data Owner"@en ;
    rdfs:comment "Core participant owning the legal rights for, and having complete control over, the data it makes available in the Industrial Data Space; defines the terms and conditions of use of its data."@en .

ids:DataProvider
    rdfs:subClassOf ids:Role; # ids:Agent
    rdfs:label "Data Provider"@en ;
    rdfs:comment "Core participant exposing Data Sources via a Connector; a Data Provider may be an enterprise or other organization, a data marketplace, an individual, or a “smart thing”."@en .

ids:DataUser
    rdfs:subClassOf ids:Role;# ids:Agent -> will become an contract assignee
    rdfs:label "Data User"@en ;
    rdfs:comment "Role of a Participant that has the legal right to use the data of a Data Sovereign as specified by the usage policy."@en .

#ids:IdentityProvider
#    rdfs:subClassOf ids:Role;
#    rdfs:label "Identity Provider"@en ;
#    rdfs:comment "Intermediary offering services to create, maintain, manage and validate identity information of and for participants in the Industrial Data Space."@en .

